Cleanup: List does work!

theories/Dot/examples/typingExamplesUnst.v
@@ -698,13 +698,64 @@ Proof.
   apply (Subs_typed_nocoerce 𝐍); tcrush.
 Qed.
 
+Notation shiftV v := v.[ren (+1)].
+
 Section listLib.
-Context Γ.
-(* bool : boolImplT *)
-Let Γ' := boolImplT :: Γ.
 
 Definition trueTm := tskip (tproj (tv x0) "true").
 Definition falseTm := tskip (tproj (tv x0) "false").
+
+Definition nilV : vl := ν {@ (* self => *)
+  type "A" = ⊥;
+  val "isEmpty" = vabs (* d => *) (trueTm.|[ren (+2)]); (* for self and d *)
+  val "head" = vabs loopTm;
+  val "tail" = vabs loopTm
+}.
+
+(*
+  λ(x: {A})λ(hd: x.A)λ(tl: sci.List∧{A <: x.A}) let result = ν(self) {
+    A = x.A; isEmpty = bool.false; head = hd; tail = tl } in result *)
+Definition consV : vl :=
+  vabs (* x => *) $ vabs' (* hd => *) $ vabs' (* tl => *) $ tv $ ν {@ (* self => *)
+    type "A" = p3 @; "T";
+    val "isEmpty" = vabs (* d => *) falseTm.|[ren (+5)];
+    val "head" = vabs (* d => *) (tv x3);
+    val "tail" = vabs (* d => *) (tv x2)
+  }.
+
+Definition listTBodyGen L U := μ {@ (* self => *)
+  type "A" >: shift L <: shift U;
+  val "isEmpty" : ⊤ →: p2 @; "Boolean"; (* bool.Boolean *)
+  val "head" : ⊤ →: p0 @; "A"; (* self.A *)
+  val "tail" : ⊤ →: TAnd (p1 @; "List") (type "A" >: ⊥ <: p0 @; "A" )
+}.
+
+Definition listTBody := listTBodyGen ⊥ ⊤.
+
+Definition listV : vl := ν {@ (* sci => *)
+  type "List" = listTBody; (* [shift] is for [sci] *)
+  val "nil" = shiftV nilV;
+  val "cons" = shiftV consV
+}.
+
+Definition nilT := TAnd listTBody (typeEq "A" ⊥).
+
+(** ∀(x: {A})∀(hd: x.A)∀(tl: sci.List∧{A <: x.A})sci.List∧{A <: x.A} *)
+Definition consT sci : ty :=
+  TAll (tparam "T")
+    (p0 @; "T" →:
+    (TAnd (shift sci @; "List") (type "A" >: ⊥ <: p0 @; "T")) →:
+    TAnd (shift sci @; "List") (type "A" >: ⊥ <: p0 @; "T")).
+
+Definition listT : ty := μ {@ (* sci => *)
+  type "List" >: ⊥ <: listTBody; (* [shift] is for [sci] *)
+  val "nil" : nilT;
+  val "cons" : consT p0
+}.
+Context Γ.
+
+(* bool : boolImplT *)
+Let Γ' := boolImplT :: Γ.
 
 Lemma trueTyp Γ'' : Γ'' ++ Γ' u⊢ₜ trueTm.|[ren (+length Γ'')] : p0.|[ren (+length Γ'')] @; "Boolean".
 Proof.
@@ -731,164 +782,68 @@ Proof.
     (* Needed: *)
     repeat lNext.
 Qed.
-(* Definition consTResConcr U : ty := listTBodyGen U U. *)
-(* Definition consTResConcr U : ty := listTBodyGen U U. *)
-(* Eval cbv in listTBodyGen ⊥ (p0 @; "T").
-Eval cbv in (listTBodyGen ⊥ (p1 @; "T")).|[ids 1 .: ids 0 .: ids]. *)
 
-Definition listTBodyGen2 L U := μ {@ (* self => *)
-  type "A" >: shift L <: shift U;
-  val "isEmpty" : ⊤ →: p2 @; "Boolean"; (* bool.Boolean *)
-  val "head" : ⊤ →: p0 @; "A"; (* self.A *)
-  val "tail" : ⊤ →: TAnd (p1 @; "List") (type "A" >: ⊥ <: p0 @; "A" )
-}.
-Definition consTResConcr2 U : ty := listTBodyGen2 U U.
-
-Definition consTConcr2 sci : ty :=
+Definition consTResConcr U : ty := listTBodyGen U U.
+Definition consTConcr sci : ty :=
   TAll (tparam "T")
     (p0 @; "T" →:
-    TAnd (shift sci @; "List") (type "A" >: ⊥ <: p0 @; "T") →:
-    (consTResConcr2 (p2 @; "T")).|[ids 1 .: ids 2 .: ids 0 .: ids]).
+      TAnd (shift sci @; "List") (type "A" >: ⊥ <: p0 @; "T") →:
+      (* This renaming is needed because I'm inserting a local variable that isn't expected by
+      [consTResConcr] *and I'm using it in the argument*. I could also just clone *)
+      (consTResConcr (p2 @; "T")).|[ids 1 .: ids 2 .: ids 0 .: ids]).
 
-Eval cbv in consTConcr2 p0.
-
-Definition listTBodyGen L U := μ {@ (* self => *)
-  type "A" >: shift L <: shift U;
-  val "isEmpty" : ⊤ →: p2 @; "Boolean"; (* bool.Boolean *)
-  val "head" : ⊤ →: p0 @; "A"; (* self.A *)
-  val "tail" : ⊤ →: TAnd (p1 @; "List") (type "A" >: ⊥ <: p0 @; "A" )
-}.
-
-Definition listTBody := Eval hnf in listTBodyGen ⊥ ⊤.
-Print listTBody.
-
-Definition nilTConcr : ty := listTBodyGen ⊥ ⊥.
-Definition nilT := TAnd listTBody (typeEq "A" ⊥).
-(* XXX reorder *)
 Definition listTConcrBody : ty := {@ (* sci => *)
   typeEq "List" $ listTBody; (* [shift] is for [sci] *)
   val "nil" : nilT;
-  val "cons" : consTConcr2 p0
+  val "cons" : consTConcr p0
 }.
+
 Definition listTConcr : ty := μ listTConcrBody.
 
-Definition nilV : vl := ν {@ (* self => *)
-  type "A" = ⊥;
-  val "isEmpty" = vabs (* d => *) (trueTm.|[ren (+2)]); (* for self and d *)
-  val "head" = vabs loopTm;
-  val "tail" = vabs loopTm
-}.
+Definition nilTConcr : ty := listTBodyGen ⊥ ⊥.
 
 Example nilTyp : (▶ listTConcrBody)%ty :: Γ' u⊢ₜ shift (tv nilV) : nilT.
 Proof.
-  cbv.
   apply (Subs_typed_nocoerce nilTConcr).
   - evar (T : ty).
     have := trueTyp [⊤; T; ▶ listTConcrBody]%ty.
     have := loopTyp (⊤ :: T :: ▶ listTConcrBody :: Γ')%ty.
-    rewrite {}/T/= => Ht Hl. cbv.
+    rewrite {}/T/= => Ht Hl.
     tcrush; apply (Subs_typed_nocoerce ⊥); tcrush.
   - tcrush.
     lThis.
     apply Bind1; tcrush.
 Qed.
-(* ∀(x: {A})∀(hd: x.A)∀(tl: sci.List∧{A <: x.A})sci.List∧{A <: x.A} *)
-
-(* Definition consTConcr sci : ty :=
-  TAll (tparam "T")
-    (p0 @; "T" →:
-    TAnd (shift sci @; "List") (type "A" >: ⊥ <: p0 @; "T") →:
-    (consTResConcr (p1 @; "T")).|[ids 1 .: ids 0 .: ids]). *)
-(* .|[upn 1 (ren (+1))] *)
-
-Definition consT sci : ty :=
-  TAll (tparam "T")
-    (p0 @; "T" →:
-    (TAnd (shift sci @; "List") (type "A" >: ⊥ <: p0 @; "T")) →:
-    TAnd (shift sci @; "List") (type "A" >: ⊥ <: p0 @; "T")).
-(*
-  λ(x: {A})λ(hd: x.A)λ(tl: sci.List∧{A <: x.A}) let result = ν(self) {
-  A = x.A; isEmpty = bool.false; head = hd; tail = tl } in result *)
-Definition consV : vl :=
-  vabs (* x => *) $ vabs' (* hd => *) $ vabs' (* tl => *) $ tv $ ν {@ (* self => *)
-    type "A" = p3 @; "T";
-    val "isEmpty" = vabs (* d => *) falseTm.|[ren (+5)];
-    val "head" = vabs (* d => *) (tv x3);
-    val "tail" = vabs (* d => *) (tv x2)
-  }.
 
 Example consTyp :
-  (▶ listTConcrBody)%ty :: Γ' u⊢ₜ shift (tv consV) : consTConcr2 p0.
+  (▶ listTConcrBody)%ty :: Γ' u⊢ₜ shift (tv consV) : consTConcr p0.
 Proof.
-  cbv.
-(* Eval cbv in (consTResConcr (p1 @; "T")).|[ids 1 .: ids 0 .: ids]. *)
   epose proof falseTyp [_; _; _; _; _; _] as Ht; cbn in Ht.
-  (* evar (T : ty).
-  have HT := falseTyp [⊤%ty; T; ▶ listTConcrBody]%ty. *)
   tcrush; clear Ht; first by varsub; eapply (LSel_stp' _ (p4 @; "T")); tcrush; varsub; lThis.
-  cbv; hideCtx. varsub. cbn. tcrush. lNext.
+  hideCtx. varsub. cbn. tcrush. lNext.
   eapply LSel_stp'; tcrush. varsub. lThis.
 Qed.
 
-Lemma consTSub : listTConcrBody :: Γ' u⊢ₜ consTConcr2 p0, 0 <: consT p0, 0.
+Lemma consTSub : listTConcrBody :: Γ' u⊢ₜ consTConcr p0, 0 <: consT p0, 0.
 Proof.
-  cbv.
   tcrush; rewrite !iterate_S !iterate_0; hideCtx.
-  2: {
-    apply Bind1; stcrush. lThis.
-  }
   eapply LSel_stp'; tcrush. varsub. tcrush. lThis.
   by lThis.
+  apply Bind1; stcrush. by lThis.
 Qed.
-  (* repeat lNext.
-  repeat lNext.
-  cbn. simplSubst.
-  rewrite !iterate_0.
-  do 3 lNext. cbn. simplSubst.
-  lThis. rewrite !iterate_S !iterate_0.
-  tcrush.
-  (* rewrite /consT /consTConcr /consTResConcr.
-  tcrush. apply Bind1; tcrush.
-  cbv; hideCtx.
-  eapply LSel_stp'; stcrush. *)
-  (* varsub. *)
-Admitted. *)
-
-
-Notation shiftV v := v.[ren (+1)].
-Definition listV : vl := ν {@ (* sci => *)
-  type "List" = listTBody; (* [shift] is for [sci] *)
-  val "nil" = shiftV nilV;
-  val "cons" = shiftV consV
-}.
-
-Definition listT : ty := μ {@ (* sci => *)
-  type "List" >: ⊥ <: listTBody; (* [shift] is for [sci] *)
-  val "nil" : nilT;
-  val "cons" : consT p0
-}.
 
 Example listTypConcr : Γ' u⊢ₜ tv listV : listTConcr.
 Proof.
-  have := nilTyp.
-  move => *.
-  apply VObj_typed; stcrush.
-  typconstructor; [ tcrush | | tcrush].
-  typconstructor; [ tcrush | | tcrush].
-  have := consTyp => *.
-  typconstructor; [ | tcrush | tcrush].
-  by apply dvl_typed.
+  have := nilTyp => *.
+  (* Without the call to [dvl_typed], Coq would (smartly) default to [dvabs_typed] *)
+  have := consTyp => /(dvl_typed "cons") *.
+  tcrush.
 Qed.
 
 Example listTyp : Γ' u⊢ₜ tv listV : listT.
 Proof.
-  have := listTypConcr.
-  have := consTSub.
-  (* have := consTyp. *)
-  (* have := nilTyp. *)
-  move => *.
-  (* evar (U : ty); have := nilTyp U; rewrite {}/U => Ht. *)
-
+  have Hv := listTypConcr.
+  have Hsub := consTSub.
   apply (Subs_typed_nocoerce listTConcr); tcrush.
   lThis.
   lNext.
